soundness proof

double_anno_inter/coq/misc/cpdt3.v
@@ -65,4 +65,129 @@ Definition tl A (s : stream A) : stream A :=
     | Cons _ _ s' => s'
     end.
 
-CoFixpoint bad : stream nat := tl nat (Cons nat 0 bad).
+(*CoFixpoint bad : stream nat := bad.*)
+
+(*
+Infinite Proofs
+*)
+
+CoFixpoint ones : stream nat := Cons nat 1 ones.
+
+Definition ones' := map nat nat S zeroes.
+
+Section stream_eq.
+  Variable A : Type.
+
+  CoInductive stream_eq : stream A -> stream A -> Prop :=
+  | Stream_eq : forall h t1 t2,
+    stream_eq t1 t2 ->
+    stream_eq (Cons A h t1) (Cons A h t2).
+
+End stream_eq.
+
+Theorem ones_eq : stream_eq nat ones ones'.
+cofix ones_eq.
+assumption.
+Undo.
+simpl.
+Abort.
+
+Definition frob A (s : stream A) : stream A :=
+    match s with
+    | Cons _ h t => Cons A h t
+    end.
+
+Theorem  frob_eq : forall A (s : stream A), s = frob A s.
+Proof.
+    destruct s. reflexivity.
+Qed.
+
+Theorem ones_eq : stream_eq nat ones ones'.
+Proof.
+    cofix ones_eq.
+    rewrite (frob_eq nat ones).
+    rewrite (frob_eq nat ones').
+    simpl.
+    constructor.
+    assumption.
+Guarded.
+Qed.
+
+Theorem ones_eq' : stream_eq nat ones ones'.
+Proof.
+    cofix one_eq'; auto.
+Abort.
+
+Definition hd A (s : stream A) : A :=
+    match s with
+    | Cons _ x _ => x
+    end.
+
+Section stream_eq_coind.
+  Variable A : Type.
+  Variable R : stream A -> stream A -> Prop.
+
+Hypothesis Cons_case_hd : forall s1 s2, R s1 s2 -> hd A s1 = hd A s2.
+Hypothesis Cons_case_tl : forall s1 s2, R s1 s2 -> R (tl A s1) (tl A s2).
+
+
+Theorem stream_eq_coind : forall s1 s2, R s1 s2 -> stream_eq A s1 s2.
+cofix stream_eq_coind; destruct s1; destruct s2; intro.
+Admitted.
+End stream_eq_coind.
+
+Require Import Arith.
+
+(*
+Simple Modeling of Non-Terminating Programs
+*)
+
+Definition var := nat.
+
+Definition vars := var -> nat.
+Definition set (vs : vars) (v : var) (n : nat) : vars :=
+    fun v' => if beq_nat v v' then n else vs v'.
+
+Inductive exp : Set :=
+| Const : nat -> exp
+| Var : var -> exp
+| Plus : exp -> exp -> exp.
+
+Fixpoint evalExp (vs : vars) (e : exp) : nat :=
+    match e with
+    | Const n => n
+    | Var v => vs v
+    | Plus e1 e2 => evalExp vs e1 + evalExp vs e2
+    end.
+
+Inductive cmd : Set :=
+| Assign : var -> exp -> cmd
+| Seq : cmd -> cmd -> cmd
+| While : exp -> cmd -> cmd.
+
+CoInductive evalCmd : vars -> cmd -> vars -> Prop :=
+| EvalAssign : forall vs v e, evalCmd vs (Assign v e) (set vs v (evalExp vs e))
+| EvalSeq : forall vs1 vs2 vs3 c1 c2, evalCmd vs1 c1 vs2
+  -> evalCmd vs2 c2 vs3
+  -> evalCmd vs1 (Seq c1 c2) vs3
+| EvalWhileFalse : forall vs e c, evalExp vs e = 0
+  -> evalCmd vs (While e c) vs
+| EvalWhileTrue : forall vs1 vs2 vs3 e c, evalExp vs1 e <> 0
+  -> evalCmd vs1 c vs2
+  -> evalCmd vs2 (While e c) vs3
+  -> evalCmd vs1 (While e c) vs3.
+
+  Section evalCmd_coind.
+  Variable R : vars -> cmd -> vars -> Prop.
+
+  Hypothesis AssignCase : forall vs1 vs2 v e, R vs1 (Assign v e) vs2
+    -> vs2 = set vs1 v (evalExp vs1 e).
+
+  Hypothesis SeqCase : forall vs1 vs3 c1 c2, R vs1 (Seq c1 c2) vs3
+    -> exists vs2, R vs1 c1 vs2 /\ R vs2 c2 vs3.
+
+  Hypothesis WhileCase : forall vs1 vs3 e c, R vs1 (While e c) vs3
+    -> (evalExp vs1 e = 0 /\ vs3 = vs1)
+    \/ exists vs2, evalExp vs1 e <> 0 /\ R vs1 c vs2 /\ R vs2 (While e c) vs3.
+
+End evalCmd_coind.
